src/typechecker/FStar.TypeChecker.Env.fst
@@ -1853,6 +1853,12 @@ let uvars_for_binders env (bs:S.binders) substs add_guard_uvars reason r =
       | _, t::_ -> Some (Ctx_uvar_meta_attr t), Some (Ctx_uvar_meta_attr t)
       | _ -> None, None in
 
+    let add_guard_uvars =
+      add_guard_uvars &&
+      (match ctx_uvar_meta_t with
+       | Some (Ctx_uvar_meta_attr _) -> not (Options.admit_tactic_unification_guards ())
+       | _ -> true) in
+
     let guard_uvar_tms, guard_uvar_opt, g_guard_uvar =
       if add_guard_uvars
       then let t, [u, _], g = new_implicit_var_with_kind
